\documentclass{article}
\usepackage{homework-preamble}

\title{CAP: Homework 6 (Workshop 71)}
\author{Franz Miltz (UNN: S1971811)}
\begin{document}
\maketitle
\section*{Question 1}
We need to find the height $h(t)$ at $t$ seconds after liftoff:
\begin{align*}
  h(t) = \int_0^t v(t)\: dt.
\end{align*}
We can solve the indefinite integral easily:
\begin{align*}
  \int v(t)\:dt & = \int \left(-gt -v_e \ln \left(\frac{m-rt}{m}\right)\right)\:dt \\
                & = -g \int t\: dt -v_e \int \ln\left(1-\frac{r}{m}t\right)\: dt   \\
                & =-\frac{1}{2}gt^2-v_e \int \ln\left(1-\frac{r}{m}t\right)\:dt.
\end{align*}
For the second part we can let $u=1-\frac{r}{m}t$  and  $du = -\frac{r}{m}dt$. This gives
\begin{align*}
  \int\ln\left(1-\frac{r}{m}t\right)\: dt = -\frac{m}{r}\int \ln u\: du = -\frac{m}{r}\left(\left(1-\frac{r}{m}t\right)\ln\left(1-\frac{r}{m}t\right)-1+\frac{r}{m}t\right)+C'.
\end{align*}
The original integral therefore is
\begin{align*}
  \int v(t)dt =-\frac{1}{2}gt^2+\frac{mv_e}{r}\left(\left(1-\frac{r}{m}t\right)\ln\left(1-\frac{r}{m}t\right)+\frac{r}{m}t\right)+C.
\end{align*}
Since I combined the constants into $C$, this is $0$ at $t=0$ with $C=0$. Thus the formula for $h(t)$ is
\begin{align*}
  h(t)=562500\left(\left(1-\frac{2}{375}t\right)\ln\left(1-\frac{2}{375}t\right)+\frac{2}{375}t\right) -4.9\cdot t^2
\end{align*}
and therfore the height above ground of the rocket one minute after liftoff in metres $h(60)$ is
\begin{align*}
  h(60)=14844.1.
\end{align*}
\section*{Question 2}
\subsection*{a)}
We will first evaluate the definite integral $I$:
\begin{align*}
  I(t)=\int \sqrt{t}\ln t\: dt.
\end{align*}
Using integration by parts with
\begin{align*}
  \begin{aligned}
    u  & = \ln t           \\
    du & = \frac{1}{t}\:dt
  \end{aligned}
  \hspace{1cm}
  \begin{aligned}
    dv & = \sqrt{t}\:dt                   \\
    v  & = \frac{2}{3}t^{\nicefrac{3}{2}}
  \end{aligned}
\end{align*}
we get
\begin{align*}
  I(t) & =\frac{2}{3}t^{\nicefrac{3}{2}}\ln t - \frac{2}{3}\int \sqrt{t}\:dt \\
       & =\frac{2}{3}t^{\nicefrac{3}{2}}(\ln t - \frac{2}{3}) + C.
\end{align*}
We can evaluate this at $t=1$ and $t=4$:
\begin{align*}
  I(1) & =\frac{2}{3}\cdot 1\cdot (0-\frac{2}{3})+C=-\frac{4}{9}+C,                           \\
  I(4) & =\frac{2}{3}\cdot 8\cdot(\ln 4 - \frac{2}{3})+C=\frac{16}{3}(\ln 4 - \frac{2}{3})+C.
\end{align*}
Thus we can find the value of the original integral:
\begin{align*}
  \int_1^4 \sqrt{t}\ln t\:dt & = I(4)-I(1)                                       \\
                             & =\frac{16}{3}\ln 4 - \frac{28}{4}                 \\
                             & = \frac{4}{3}(8\ln 2 - \frac{7}{3})\approx 4.282.
\end{align*}
\subsection*{b)}
At first, we can use the quality
\begin{align*}
  \tan^2 x = \sec^2 x - 1
\end{align*}
to simplify the integral:
\begin{align*}
  I & = \int \tan^2 x \sec x\:dx
  = \int (\sec^2 x - 1)\sec x\:dx            \\
    & = \int \sec^3 x\:dx  - \int \sec x\:dx
\end{align*}
We know
\begin{align}
  \label{eq:1}
  \int \sec x\: dx = \ln |\sec x + \tan x| + C_1.
\end{align}
Let's evaluate the other integral. We use integration by parts with
\begin{align*}
  \begin{aligned}
    u  & = \sec x             \\
    du & = \sec x \tan x\: dx
  \end{aligned}
  \hspace{1cm}
  \begin{aligned}
    dv & = \sec^2 x\: dx \\
    v  & = \tan x
  \end{aligned}
\end{align*}
to get
\begin{align*}
  I'=\int \sec^3 x \: dx & =\sec x\tan x - \int \sec x \tan^2 x\: dx        \\
                         & = \sec x \tan x - \int \sec x (\sec^2 x - 1)\:dx \\
                         & = \sec x \tan x - I' + \int \sec x \: dx.
\end{align*}
Using equation \ref{eq:1}, we can solve for $I'$ to get
\begin{align*}
  I'=\frac{1}{2}(\sec x \tan x + \ln |\sec x + \tan x|) + C_2.
\end{align*}
Thus we conclude that
\begin{align*}
  I=\frac{1}{2}(\sec x \tan x -\ln |\sec x + \tan x|) + C.
\end{align*}
\subsection*{c)}
To solve the integral
\begin{align*}
  I(r) & = \int \frac{r^3}{\sqrt{4+r^2}}dr,
\end{align*}
we use the subsitution
\begin{align*}
  u = 4+r^2 \hspace{1cm}  du = 2rdr.
\end{align*}
Thus we get
\begin{align*}
  I(r) & = \frac{1}{2}\int \frac{u-4}{\sqrt{u}}\:du                    \\
       & =\frac{1}{2}\int\sqrt{u}\:du - 2 \int \frac{1}{\sqrt{u}}\:du.
\end{align*}
We can solve those two integrals easily using the power rules:
\begin{align*}
  \int \sqrt{u}\:du           & =\frac{2}{3}u^{\nicefrac{3}{2}}+C_1, \\
  \int \frac{1}{\sqrt{u}}\:du & =2\sqrt{u}+C_2.
\end{align*}
Therefore
\begin{align*}
  I(r) = \frac{1}{3}u^{\nicefrac{3}{2}}-4\sqrt{u}+C.
\end{align*}
Substituting $u=r^2+4$ gives
\begin{align*}
  I(r) & = \frac{1}{3}(4+r^2)^{\nicefrac{3}{2}}-4\sqrt{4+r^2} + C \\
       & = \frac{1}{3}(r^2-8)\sqrt{4+r^2}+C.
\end{align*}
Now we can evaluate at $r=0$ and $r=1$:
\begin{align*}
  I(0) & =\frac{1}{3}(0-8)\sqrt{4+0}+C=-\frac{16}{3}+C         \\
  I(1) & =\frac{1}{3}(1-8)\sqrt{4+1}+C=-\frac{7\sqrt{5}}{3}+C.
\end{align*}
Therefore we get
\begin{align*}
  \int_0^1\frac{r^3}{\sqrt{4+r^2}}\:dr = \frac{16-7\sqrt{5}}{3} \approx 0.116.
\end{align*}
\subsection*{d)}
To solve
\begin{align*}
  I(x)=\int e^{\sqrt{x}}\:dx
\end{align*}
we can use
\begin{align*}
  u=\sqrt{x}\hspace{1cm}du=\frac{1}{2\sqrt{x}}
\end{align*}
to get
\begin{align*}
  I(x)=2\int ue^u\:du.
\end{align*}
Now we can integrate by parts with
\begin{align*}
  \begin{aligned}
    f  & = u  \\
    df & = du
  \end{aligned}
  \hspace{1cm}
  \begin{aligned}
    dg & = e^u\: du \\
    g  & = e^u
  \end{aligned}
\end{align*}
to get
\begin{align*}
  I(x)=2ue^u-2\int e^udu=2(u-1)e^u+C.
\end{align*}
Undoing the subsitution $u=\sqrt{x}$, we get
\begin{align*}
  \int e^{\sqrt{x}}dx = I(x)=2(\sqrt{x}-1)e^{\sqrt{x}}+C.
\end{align*}
Evaluating at $x=0$ and $x=1$ gives
\begin{align*}
  I(0)=2\cdot(0-1)\cdot 1+C=-2+C, \\
  I(1)=2\cdot(1-1)\cdot e^1+C=0+C.
\end{align*}
Thus
\begin{align*}
  \int_0^1 e^{\sqrt{x}}\: dx = 0 - (-2) = 2.
\end{align*}
\end{document}