\documentclass{article}
\usepackage{homework-preamble}

\begin{document}
\title{Geometry: Hand-in 4}
\author{Franz Miltz (UUN: S1971811)}
\date{22 November 2021}
\maketitle
\noindent Let $D=\{u,v,z\in\R : u,v\not=0\}$ and let $\vec x:D\to\E^3$ be such that
\begin{align*}
   \vec x(u,v,z) = \begin{pmatrix}
      uv \\ \frac{1}{2}(v^2 - u^2) \\ z
   \end{pmatrix}
\end{align*}

\section*{Question 1}

\begin{claim*}
   \begin{align}
      \label{dx}
      d\vec x = \sqrt{u^2 + v^2}du\vec e_1
      + \sqrt{u^2 + v^2}dv \vec e_2
      + dz\vec e_3
   \end{align}
   where
   \begin{align*}
      \vec e_1 = \frac{1}{\sqrt{u^2 + v^2}}\begin{pmatrix}
         v \\ -u \\ 0
      \end{pmatrix} , \hs
      \vec e_2 = \frac{1}{\sqrt{u^2 + v^2}}\begin{pmatrix}
         u \\ v \\ 0
      \end{pmatrix}, \hs
      \vec e_3 = \begin{pmatrix}
         0 \\ 0 \\ 1
      \end{pmatrix}
   \end{align*}
   are a moving frame on $D$.
\end{claim*}
\begin{proof}
   Firstly, we calculate
   \begin{align*}
      d\vec x = \begin{pmatrix}
         v du + u dv  \\
         -u du + v dv \\
         dz
      \end{pmatrix}.
   \end{align*}
   It's straightforward to verify algebraically that (\ref{dx}) holds. Secondly,
   we note that $u,v\not=0$ and therefore that the $\vec e_i$ are well-defined on $D$
   and smooth. Lastly, we observe that
   \begin{align}
      \vec e_i \cdot \vec e_j = \delta_i^j,
   \end{align}
   making $\{\vec e_1, \vec e_2, \vec e_3\}$ a moving frame.
\end{proof}

\section*{Question 2}

\begin{claim*}
   The connection 1-forms are
   \begin{align*}
      \omega_2^1 = \frac{vdu - udv}{u^2 + v^2},\hs
      \omega_3^1 = \omega_3^2 = 0.
   \end{align*}
\end{claim*}
\begin{proof}
   We begin by computing
   \begin{align*}
      d\vec e_2 = \frac{1}{(u^2+v^2)^{3/2}}\begin{pmatrix}
         v^2du - uvdv   \\
         - uvdu + u^2dv \\
         0
      \end{pmatrix}.
   \end{align*}
   This lets us determine
   \begin{align*}
      \omega_2^1 = \vec e_1 \cdot d\vec e_2 = \frac{vdu - udv}{u^2 + v^2}.
   \end{align*}
   Finally, we note that $d\vec e_3 = \vec 0$ and thus
   \begin{align}
      \label{omega0}
      \omega_3^1 = \vec e_1 \cdot d\vec e_3=0, \hs \omega_3^2 = \vec e_2 \cdot d\vec e_3=0.
   \end{align}
\end{proof}

\begin{claim*}
   The structure equations,
   \begin{align}
      \label{se1}
      d\theta^1 + \omega_2^1 \wedge \theta^2 = 0,              \\
      \label{se2}
      d\theta^2 + \omega_1^2 \wedge \theta^1 = 0,              \\
      \label{se3}
      \omega_1^3\wedge\theta^1 + \omega_2^3\wedge\theta^2 = 0, \\
      \label{se4}
      d\omega_2^1+\omega_3^1 \wedge\omega_2^3 = 0,             \\
      \label{se5}
      d\omega_3^1 + \omega_2^1 \wedge \omega_3^2 = 0,          \\
      \label{se6}
      d\omega_3^2 + \omega_1^2 \wedge \omega_3^1 = 0,
   \end{align}
   are satisfied.
\end{claim*}
\begin{proof}
   Consider (\ref{se1}). We compute
   \begin{align*}
      d\theta^1 = \frac{v}{\sqrt{u^2+v^2}}dv\wedge du,\hs
      \omega_2^1 \wedge \theta^2 = \frac{v}{\sqrt{u^2+v^2}}du\wedge dv.
   \end{align*}
   Since $dv\wedge du = - du \wedge dv$, the equation holds.
   Consider (\ref{se2}). We compute
   \begin{align*}
      d\theta^2 = \frac{u}{\sqrt{u^2+v^2}}du\wedge dv, \hs
      \omega_1^2 \wedge \theta^1 = - \frac{u}{\sqrt{u^2 + v^2}}du\wedge dv
   \end{align*}
   where we used $\omega_1^2 = - \omega_2^1$. The equation clearly holds.
   Now we observe that (\ref{se3}), (\ref{se5}) and (\ref{se6}) depend on
   $\omega_3^2=\omega_3^1=0$ in such a way that they are trivially satisfied.
   Further, (\ref{se4}) simplifies to
   \begin{align*}
      d\omega_2^1 = 0.
   \end{align*}
   We calculate
   \begin{align*}
      d\omega_2^1 = \frac{u^2-v^2}{u^2+v^2}dv\wedge du + \frac{u^2-v^2}{u^2+v^2}du\wedge dv.
   \end{align*}
   Again, by $dv\wedge du = - du \wedge dv$ this clearly holds.
\end{proof}

\end{document}