\documentclass{article}
\usepackage{homework-preamble}

\begin{document}
\title{Geometry: Hand-in 1}
\author{Franz Miltz (UUN: S1971811)}
\date{11 October 2021}
\maketitle

\begin{claim*}[Question 1]
	Let $\vec x: I\to \E^3$ be the space curve given by
	\begin{align*}
		\vec x(s) = \begin{pmatrix}
			            \frac{\sqrt{3}}{2}\sin s \\
			            \cos s                   \\
			            \frac{1}{2}\sin s
		            \end{pmatrix}.
	\end{align*}
	Then
	\begin{align*}
		v(s) = 1, \kappa(s) = 1, \tau(s) = 0, \\
	\end{align*}
	and
	\begin{align*}
		\{\vec T(s), \vec N(s), \vec B(s)\} =
		\left\lbrace  \begin{pmatrix}
			              \frac{\sqrt{3}}{2}\cos s \\
			              - \sin s                 \\
			              \frac{1}{2}\cos s
		              \end{pmatrix}, \begin{pmatrix}
			                             -\frac{\sqrt{3}}{2}\sin s \\
			                             - \cos s                  \\
			                             -\frac{1}{2}\sin s
		                             \end{pmatrix}, \begin{pmatrix}
			                                            1/2 \\ 0 \\ \sqrt{3}/2
		                                            \end{pmatrix}
		\right\rbrace
	\end{align*}
	for all $s\in I$.
\end{claim*}
\begin{proof}
	We have
	\begin{align*}
		\vec x'(s) = \begin{pmatrix}
			             \frac{\sqrt{3}}{2}\cos s \\
			             - \sin s                 \\
			             \frac{1}{2}\cos s
		             \end{pmatrix},\hs
		\vec x''(s) = \begin{pmatrix}
			              -\frac{\sqrt{3}}{2}\sin s \\
			              - \cos s                  \\
			              -\frac{1}{2}\sin s
		              \end{pmatrix}.
	\end{align*}
	Therefore
	\begin{align*}
		v(s) = \abs{x'(s)}       & = \frac{3}{4}\cos^2 s + \sin^2 s + \frac{1}{4}\cos^2 s = 1, \\
		\kappa(s) = \abs{x''(s)} & = \frac{3}{4}\sin^2 s + \cos^2 s + \frac{1}{4}\cos^2 s = 1.
	\end{align*}
	Since $v(s)=1$ we have $\vec T(s)=\vec x'(x)$. Further, since
	$\vec T'(s)=\vec x''(s)$,
	\begin{align*}
		\vec N(s) = \frac{\vec T'(s)}{\abs{\vec T'(s)}} = \vec x''(s).
	\end{align*}
	Finally,
	\begin{align*}
		\vec B (s) = \vec T(s) \times \vec N(s) = \begin{pmatrix}
			                                          1/2 \\ 0 \\ \sqrt{3}/2
		                                          \end{pmatrix}.
	\end{align*}
	This allows us to compute the torsion $\tau$,
	\begin{align*}
		\tau(s) = -\vec B'(s) \cdot \vec N(s) = \vec 0 \cdot \vec N(s) = 0.
	\end{align*}
	The Frenet-Serret frame is given by the vectors
	\begin{align*}
		\vec T(s) = \begin{pmatrix}
			            \frac{\sqrt{3}}{2}\cos s \\
			            - \sin s                 \\
			            \frac{1}{2}\cos s
		            \end{pmatrix},\:
		\vec N(s)=\begin{pmatrix}
			          -\frac{\sqrt{3}}{2}\sin s \\
			          - \cos s                  \\
			          -\frac{1}{2}\sin s
		          \end{pmatrix}, \:
		\vec B(s) = \begin{pmatrix}
			            1/2 \\ 0 \\ \sqrt{3}/2
		            \end{pmatrix}.
	\end{align*}
\end{proof}

\begin{claim*}[Question 2.1]
	Let $\vec x : I \to \E^n$ be a unit-speed parameterised curve such that
	\begin{align}
		\label{premise}
		\abs{\vec x(s) - \vec p}^2 = R^2 \hs\text{for all } s\in I
	\end{align}
	where $R\in\R$ and $\vec p\in\E^n$. Then $\kappa(s)\geq 1/R$ for all $s\in I$.
\end{claim*}
\begin{proof}
	We differentiate (\ref{premise}) with respect to $s$ to obtain
	\begin{align*}
		\vec x'(s) \cdot (\vec x(s) - \vec p) = 0.
	\end{align*}
	Doing this again yields
	\begin{align}
		\label{d2}
		\vec x''(s)\cdot (\vec x(s) - \vec p) + \vec x'(s)\cdot\vec x'(s) = 0.
	\end{align}
	Note that $\vec x(s)$ is unit-speed parameterised and therefore
	\begin{align*}
		\vec x'(s) = \vec T(s), \hs \abs{\vec x'(s)} = 1.
	\end{align*}
	We use this to simplify (\ref{d2}) to
	\begin{align}
		\label{t}
		\vec T'(s) \cdot (\vec x(s) - \vec p) + 1 = 0.
	\end{align}
	Therefore, $\vec T'(s)\not= \vec 0$, making $\vec x$ biregular. This allows
	us to use the structure equations to obtain
	\begin{align*}
		\kappa(s)\vec N(s)\cdot(\vec x(s)-\vec p) + 1 = 0
	\end{align*}
	which, since $\vec N(s)\cdot(\vec x(s)-\vec p)$ is clearly nonzero, we
	can rearrange as follows
	\begin{align*}
		\kappa(s)=-\frac{1}{\vec N(s)\cdot(\vec x(s) - \vec p)}.
	\end{align*}
	However, we know that $\kappa(s)>0$ for all $s$. Thus
	\begin{align}
		\label{curvature}
		\kappa(s) = \frac{1}{\abs{\vec N(s)\cdot(\vec x(s)-\vec p)}}.
	\end{align}
	By the \emph{Cauchy-Schwarz inequality} we have
	\begin{align*}
		0 < \abs{\vec N(s)\cdot(\vec x(s) - \vec p)} \leq \abs{\vec N(s)}\abs{\vec x(s)-\vec p}.
	\end{align*}
	Observe that $\abs{\vec N(s)} = 1$, $\abs{\vec x(s) - \vec p} = R$ and thereby
	\begin{align*}
		0 <\abs{\vec N(s) \cdot (\vec x(s) - \vec p)} \leq R
	\end{align*}
	which shows
	\begin{align*}
		\kappa(s) \geq \frac{1}{R}.
	\end{align*}
\end{proof}

\begin{claim*}[Question 2.2]
	Let $\vec x : I \to \E^n$ be a unit-speed parameterised curve such that
	\begin{align*}
		\abs{\vec x(s) - \vec p}^2 = R^2,\hs\kappa(s)=c \hs\text{for all } s\in I
	\end{align*}
	where $c, R\in\R$ and $\vec p\in\E^n$.
	Then $\vec x(s)$ is part of a circle.
\end{claim*}
\begin{proof}
	In the proof above we have established that
	\begin{align*}
		\kappa(s)\vec N(s)\cdot (\vec x(s)-\vec p) + 1 = 0.
	\end{align*}
	Since $\kappa(s)=c$, this is equivalent to
	\begin{align}
		\label{eq1}
		\vec N(s)\cdot (\vec x(s) - \vec p) + \frac{1}{c} = 0.
	\end{align}
	We can differentiate to obtain
	\begin{align*}
		\vec N'(s)\cdot (\vec x(s) - \vec p) + \vec N(s)\cdot \vec x'(s)=0.
	\end{align*}
	Since $\vec T(s) = \vec x'(s)$ and $\vec T(s) \cdot \vec N(s)=0$ by
	\emph{Notes, Proposition 3.14}, this simplifies to
	\begin{align*}
		\vec N'(s)\cdot (\vec x(s)-\vec p) = 0.
	\end{align*}
	We can use the structure equations again to get
	\begin{align*}
		(-c \vec T'(s) + \tau\vec B'(s))\cdot (\vec x(s)-\vec p) = 0.
	\end{align*}
	By differentiation this shows
	\begin{align*}
		(-c \vec T'(s) + \tau \vec B'(s)) \cdot (\vec x(s) - \vec p)
		+ (-c \vec T(s) + \tau \vec B(s)) \cdot \vec T = 0,
	\end{align*}
	which we can simplify by using $\vec T(s)\cdot \vec T(s)=1$ and $\vec B(s)\cdot \vec T(s)=0$:
	\begin{align*}
		(-c \vec T'(s) + \tau \vec B'(s)) \cdot (\vec x(s) - \vec p) = c.
	\end{align*}
	However, due to (\ref{t}), we find
	\begin{align*}
		\tau \vec B'(s)\cdot (\vec x(s) - \vec p) = 0.
	\end{align*}
	By applying the structure equations one last time, we find
	\begin{align*}
		-\tau^2 \vec N(s)\cdot (\vec x(s)-\vec p) = 0.
	\end{align*}
	Due to (\ref{eq1}), $\vec N(s)\cdot (\vec x(s)-\vec p)\not=0$, which shows $\tau=0$.
	By \emph{Notes, Corollary 3.26}, this makes $\vec x(s)$ part of a circle.
\end{proof}

\end{document}