\documentclass{article}
\usepackage{homework-preamble}

\begin{document}
\title{Geometry: Hand-in 3}
\author{Franz Miltz (UUN: S1971811)}
\date{8 November 2021}
\maketitle

\section*{Question 1}

\emph{The proof below is obviously wrong as $x^n$ may be zero,
   but I have not been able to find smooth parameters for $\beta$ that are defined everywhere.}

\begin{claim*}
   Let $\alpha\in\Omega^1(\R^n)$ be a $1$-form such that
   \begin{align*}
      \alpha=\sum_{i=1}^n x^idx^i.
   \end{align*}
   Then there exists $\beta\in\Omega^{n-1}(\R^n\setminus\{\vec 0\})$ such that
   \begin{align*}
      \alpha\wedge\beta = dx^1\wedge\cdots\wedge dx^n.
   \end{align*}
\end{claim*}
\begin{proof}
   Let
   \begin{align*}
      \beta = \frac{(-1)^{n-1}}{x^n}dx^1\wedge\cdots\wedge dx^{n-1}.
   \end{align*}
   Then we have
   \begin{align*}
      \alpha\wedge\beta & = \left(\sum_{i=1}^n x^idx^i\right) \wedge \left(\frac{(-1)^{n-1}}{x^n}dx^1\wedge\cdots\wedge dx^{n-1}\right) \\
                        & = \sum_{i=1}^n \frac{(-1)^{n-1}x^i}{x^n}dx^i\wedge dx^1 \wedge \cdots dx^{n-1}.
   \end{align*}
   However, for all $1\leq i\leq n-1$ the wedge product is zero due to the repeated $dx^i$. Thus
   \begin{align*}
      \alpha\wedge\beta = \frac{(-1)^{n-1}x^n}{x^n}dx^n\wedge dx^1\wedge\cdots\wedge dx^{n-1}=dx^1\wedge\cdots\wedge dx^n.
   \end{align*}
\end{proof}

\section*{Question 2}

Let $\vec x: D\to\E^3$ be a local surface defined by $D=\{z\in\R,\phi\in(0,2\pi)\}\subset\R^3$ and
\begin{align*}
   \vec x(z,\phi)=\begin{pmatrix}
      \cosh z \cos\phi \\ \cosh z \sin\phi \\ z
   \end{pmatrix}.
\end{align*}

\begin{claim*}
   $\vec x$ is regular and the first fundamental form is
   \begin{align*}
      I= (\cosh^2 z)(dz)^2 + (\cosh^2 z) (d\phi)^2.
   \end{align*}
\end{claim*}
\begin{proof}
   We calculate
   \begin{align}
      \label{dirderiv1}
      \vec x_z    & = \sinh z \cos\phi \frac{\p }{\p x^1}
      + \sinh z \sin\phi \frac{\p }{\p x^2}
      + \frac{\p }{\p x^3},                                \\
      \label{dirderiv2}
      \vec x_\phi & = -\cosh z \sin\phi \frac{\p }{\p x^1}
      + \cosh z\cos\phi\frac{\p }{\p x^2}.
   \end{align}
   Firstly, we observe that both $\vec x_z$ and $\vec x_\phi$ are non-zero on $D$.
   Further,
   \begin{align*}
      \vec x_z \cdot \vec x_\phi = -\sinh z\cosh z\sin\phi\cos\phi + \sinh z\cosh z\sin\phi\cos\phi
      = 0.
   \end{align*}
   Therfore $\vec x_z$ and $\vec x_\phi$ are non-zero and perpendicular everywhere, making them linearly
   independent. By definition, this shows that $\vec x$ is a regular local surface.
   Further, we have
   \begin{align*}
      (dx^1)^2 & = (\sinh z\cos\phi dz - \cosh z \sin\phi d\phi)^2                                                     \\
               & =\sinh^2 z \cos^2\phi(dz)^2
      -2\sinh z\cosh z\sin\phi\cos\phi dzd\phi+\cosh^2z\sin^2\phi(d\phi)^2,                                            \\
      (dx^2)^2 & = (\sinh z\sin\phi dz + \cosh z \cos\phi d\phi)^2                                                     \\
               & =\sinh^2 z\sin^2\phi (dz)^2 + 2\sinh z\cosh z\sin\phi\cos\phi dzd\phi + \cosh^2 z\cos^2\phi(d\phi)^2, \\
      (dx^3)^2 & =(dz)^2.
   \end{align*}
   Therefore, by definition,
   \begin{align*}
      I=d\vec x\cdot d\vec x = (\cosh^2 z)(dz)^2 + (\cosh^2 z) (d\phi)^2.
   \end{align*}
\end{proof}

\begin{claim*}
   The unit normal of $\vec x$ at a point $(z,\phi)\in D$ is
   \begin{align*}
      \vec N(z, \phi) = \frac{-\cos\phi \frac{\p }{\p x^1}-\sin\phi\frac{\p }{\p x^2}+\sinh z\frac{\p }{\p x^3}}{\cosh z}.
   \end{align*}
\end{claim*}
\begin{proof}
   By definition, we have
   \begin{align*}
      \vec N(p) = \frac{\vec x_z \times \vec x_\phi}{\abs{\vec x_z \times \vec x_\phi}}.
   \end{align*}
   We use (\ref{dirderiv1}) and (\ref{dirderiv2}) to claculate
   \begin{align*}
      \vec x_z\times \vec x_\phi = -\cosh z \cos\phi \frac{\p }{\p x^1}-\cosh z \sin\phi\frac{\p }{\p x^2}+\sinh z\cosh z \frac{\p }{\p x^3}
   \end{align*}
   and then
   \begin{align*}
      \abs{\vec x_z\times \vec x_\phi} = \sqrt{(1 + \sinh^2 z)\cosh^2 z} = \cosh^2 z.
   \end{align*}
   The claim follows after cancellation.
\end{proof}

\begin{claim*}
   The second fundamental form of $\vec x$ at a point $(z,\phi)\in D$ is
   \begin{align*}
      \I = -(dz)^2+(d\phi)^2.
   \end{align*}
\end{claim*}

\begin{proof}
   We calculate
   \begin{align*}
      dN_1 & = d\left(-\frac{\cos\phi}{\cosh z}\right) = \left(\frac{\sinh z\cos\phi}{\cosh^2z}\right)dz + \left(\frac{\sin\phi}{\cosh z}\right)d\phi,  \\
      dN_2 & = d\left(-\frac{\sin\phi}{\cosh z}\right) = \left(\frac{\sinh z\sin\phi}{\cosh^2 z}\right)dz - \left(\frac{\cos\phi}{\cosh z}\right)d\phi, \\
      dN_3 & = d\left(\frac{\sinh z}{\cosh z}\right)   = \left(\frac{1}{\cosh^2 z}\right)dz
   \end{align*}
   We use this and our calculations for $d\vec x$ to find
   \begin{align*}
      \I = -d\vec x \cdot d\vec N = -(dz)^2 +(d\phi)^2.
   \end{align*}
\end{proof}

\begin{claim*}
   The principal curvatures of $\vec x$ at $(z,\phi)\in D$ are
   \begin{align*}
      k_1 = \frac{1}{\cosh^2 z}, \hs k_2 = -\frac{1}{\cosh^2 z}
   \end{align*}
   and thus
   \begin{align*}
      H=0,\hs K=-\frac{1}{\cosh^4 z}.
   \end{align*}
\end{claim*}
\begin{proof}
   The first and second fundamental form are represented by the following
   matrices:
   \begin{align*}
      I = \begin{pmatrix}
         \cosh^2 z & 0 \\ 0 & \cosh^2 z
      \end{pmatrix}, \hs
      \I = \begin{pmatrix}
         -1 & 0 \\ 0 & 1
      \end{pmatrix}.
   \end{align*}
   Thus the principal curvatures are the solutions to the equation
   \begin{align*}
      \det(\I-kI)=0
   \end{align*}
   which holds if and only if
   \begin{align*}
      (1+k\cosh^2 z)(1-k\cosh^2 z) = 0.
   \end{align*}
   Thus $k_1=1/\cosh^2 z$ and $k_2=-1/\cosh^2 z$.
   By definition, we then have
   \begin{align*}
      H & =\frac{1}{2}(k_1+k_2)=0,      \\
      K & =k_1k_2=-\frac{1}{\cosh^4 z}.
   \end{align*}
\end{proof}

\section*{Question 3}

\begin{claim*}
   Let $\Sigma\subset\E^3$ be a regular surface, that meets a plane $P\subset\E^3$ in a
   single point $\vec p$. Then $P$ coincides with the tangent plane of $\Sigma$ at $\vec p$,
   $T_{\vec p}\Sigma$.
\end{claim*}
\begin{proof}
   Let $P$ be given by the equation
   \begin{align*}
      \vec n \cdot (\vec x - \vec p) = 0 \hs\text{for all }\vec x\in P
   \end{align*}
   where we assume without loss of generality that $\vec n$ is a unit vector. Then the
   distance of any point $\vec x\in\E^3$ the distance to $P$ is
   \begin{align*}
      D(\vec x) = \vec n \cdot (\vec x - \vec p).
   \end{align*}
   Further, since $\Sigma$ is regular, there exists a local regular surface
   $\vec y: D\subset\R^3\to \E^3$ such that $\vec p \in\vec y(D)$ and $\vec y(D)=U\cap\Sigma$
   for some open set $U\subset\R^3$.
   The distance of a point on this surface given by $(u,v)\in D$ then is
   \begin{align*}
      D(\vec y(u,v)) = \vec n \cdot (\vec y(u,v) - \vec p) =: g(u,v).
   \end{align*}
   Consider the Jacobian matrix
   \begin{align*}
      J_g =
      \begin{bmatrix}
         \frac{\p g}{\p u} & \frac{\p g}{\p v}
      \end{bmatrix}.
   \end{align*}
   Note that the $1\times1$ matrix $\left[\eval{\frac{\p g}{\p v}}{q}\right]$ is invertible
   at $q\in D$ where $\vec y(q) = \vec p$ if and only if
   \begin{align}
      \label{non_tangent}
      \eval{\frac{\p g}{\p v}}{q} = \vec n \cdot \vec y_v(q)\not= 0.
   \end{align}
   Assume, for contradiction, that $P$ does not coincide with the tangent space
   $T_{\vec p}\Sigma$. Then we know that at $q$ either
   \begin{align*}
      \vec n \cdot \vec y_u(q) \not=0, \hs\text{or}\hs \vec n \cdot \vec y_v(q) \not=0.
   \end{align*}
   This is because $\vec y$ is regular so $\vec y_u$ and $\vec y_v$ must be linearly independent
   and span $T_{\vec p} \Sigma$. Since we could reparameterise to swap $\vec y_u$ and $\vec y_v$,
   we can assume without loss of generality that the latter inequality holds.
   We therefore have (\ref{non_tangent}).

   By the \emph{Implicit Function Theorem} there must exist a function
   \begin{align*}
      \Phi : E \subset \R \to \R
   \end{align*}
   defined on an open set $E\subset \R$ such that there exists an open set $\tilde D$
   with $q\in \tilde D\subset D$ such that
   \begin{align*}
      \tilde D \cap (\R \subset \R^2) = E,
   \end{align*}
   and such that for all $\tilde q \in \tilde D$ we have
   \begin{align*}
      g(\tilde q) = g(q) \hs\Leftrightarrow\hs \tilde q = (r, \Phi(r)) \hs \text{for some $r\in E$}.
   \end{align*}
   Since $E$ is open, there exists more than one such $r$. This implies that there
   is more than one point on $\Sigma$ where the distance to $P$ is zero which contradicts the premise.
   Therefore $P$ and $T_{\vec p}\Sigma$ must coincide.
\end{proof}


\end{document}